Remove assumptions through test_z except for expensive lemma assumptions
At Nik's suggestion, some facts about disjointness and modification are
assumed because, while provable, the lemmas required to prove them lead to
very long checking times. Those assumes are left in, though with enough
resources and the right lemmas enabled, could be properly checked.

Assumptions related to left-shifting also still remain.

qtesla/code/Hacl.Impl.QTesla.fst
@@ -1666,6 +1666,18 @@ private let lemma_disjoint
     (requires disjoint ec e /\ ec_k == gsub ec (k *! params_n) params_n /\ e_k == gsub e (k *! params_n) params_n)
     (ensures disjoint ec_k e_k) = ()
 
+private let lemma_disjoint_2
+    (#t1 #t2: Type0)
+    (#n1: size_t)
+    (#n1s: size_t)
+    (#n2: size_t)
+    (k: size_t{v k + v n1s <= v n1})
+    (buf: lbuffer t1 n1)
+    (subbuf: lbuffer t1 n1s{subbuf == gsub buf k n1s})
+    (other: lbuffer t2 n2) : Lemma
+    (requires disjoint buf other)
+    (ensures disjoint subbuf other) = ()
+
 private inline_for_extraction noextract
 val qtesla_sign_update_v:
     v_: poly_k
@@ -1688,8 +1700,8 @@ let qtesla_sign_update_v v_ e pos_list sign_list =
     assert(forall (i:nat{i < v params_n * v params_k}) . bget hInit e i == bget h0 e i);
     let _, _ =
     interruptible_for (size 0) params_k
-         (fun h _ _ -> live h v_ /\ live h e /\ live h rsp /\ (bget h rsp 0 == 0l \/ bget h rsp 0 == 1l) /\
-                    modifies2 v_ rsp h0 h /\ is_e_sk h e)
+         (fun h k _ -> live h v_ /\ live h e /\ live h rsp /\ (bget h rsp 0 == 0l \/ bget h rsp 0 == 1l) /\
+                    modifies2 v_ rsp h0 h /\ is_e_sk h e /\ k <= v params_k /\ is_poly_k_montgomery_i h v_ (k * v params_n))
          (fun k ->
              let hStart = ST.get () in
              push_frame();
@@ -1703,20 +1715,23 @@ let qtesla_sign_update_v v_ e pos_list sign_list =
              assert(is_e_sk h e);
              lemma_sub_poly_is_sk h e e_k k;
              assert(is_s_sk h e_k);
-             //NS: Not sure why this is not provable
              lemma_disjoint ec e ec_k e_k k;
              assert(disjoint ec_k e_k);
-             assume(disjoint e_k pos_list);
-             assume(disjoint e_k sign_list);
+             lemma_disjoint_2 (k *! params_n) e e_k pos_list;
+             lemma_disjoint_2 (k *! params_n) e e_k sign_list;
+             assert(disjoint e_k pos_list);
+             assert(disjoint e_k sign_list);
              sparse_mul ec_k e_k pos_list sign_list;
              poly_sub_correct (index_poly v_ k) (index_poly v_ k) (index_poly ec k);
              let hSub = ST.get () in
-             assume(is_poly_k_montgomery hSub v_);
-             lemma_sub_poly_is_montgomery hSub v_ (gsub v_ (k *! params_n) params_n) k;
+             assert(is_poly_montgomery hSub (get_poly v_ k));
              rsp.(size 0) <- test_correctness (index_poly v_ k);
              let rspVal = rsp.(size 0) in 
              pop_frame(); 
              let hLoopEnd = ST.get () in
+             assert(is_poly_equal hSub hLoopEnd (get_poly v_ k));
+             assert(forall (i:nat{i < v params_n}) . is_montgomery (bget hLoopEnd (get_poly v_ k) i));
+             assert(forall (i:nat{i >= v k * v params_n /\ i < v k * v params_n + v params_n}) . bget hLoopEnd v_ i == bget hLoopEnd (get_poly v_ k) (i - v k * v params_n));
              rspVal <> 0l
          ) in
    let rspVal = rsp.(size 0) in
